capDL: introduce generic page tables
- Drawing inspiration from AARCH64, make page table object and cap types
  parametric in pt_type. This means we need only one PageTable
  type for all page table objects (page directory, page table, etc), and
  only one page table cap type to point to them.

- Use the same type/level distinction as in AARCH64, because it can
  model all situations that occur in the currently supported seL4
  architectures. In particular, all levels could use the same type
  such as in RISCV64, each level could use its own type such as for
  X64/ARM/ARM_HYP, or a mix as in AARCH64.

- Update the existing ARM/ARM_HYP capDL spec to use this scheme.

- Add a generic implementation of page tables that works for all seL4
  architectures. It only implements the "map" system call, which is the
  only page/page table invocation needed for system initialisation.
  For other system calls, return maximum nondeterminism.

- Keep the old ARM/ARM_HYP implementation and call it when the
  architecture is AARCH32 to keep the current DRefine/SysInit proofs
  (mostly) working. The proofs will need updates for the new data types
  being used, but the existing reasoning will still apply.

Signed-off-by: Gerwin Klein <gerwin.klein@proofcraft.systems>

spec/capDL/Types_D.thy
@@ -14,6 +14,7 @@
 theory Types_D
 imports
   "ASpec.VMRights_A"
+  ASpec.Machine_A
   Intents_D
   Arch_Structs_D
   "Lib.Lib"
@@ -43,6 +44,10 @@ arch_requalify_facts
   vmpage_size_simps
   pageBitsForSize_def
   pageForPageBits_def
+
+arch_requalify_types (A)
+  asid_high_len
+  asid_low_len
 
 (* A hardware IRQ number. *)
 type_synonym cdl_irq = irq
@@ -109,6 +114,13 @@ datatype cdl_frame_cap_type = Real | Fake cdl_raw_vmattrs
  * Caps have attributes such as the object they point to, the rights
  * they give the holder, or how the holder is allowed to interact with
  * the target object.
+ *
+ * Note that frame and page tables caps (and later objects) are generic in the architecture
+ * they model and parameterised in the type of object they represent (e.g. which level of
+ * page table object). Level 0 is the bottom level where page table walks end, and max_pt_level
+ * is the highest level where the root page table is. The model is essentially the same as in
+ * ASpec for AARCH64. See there for more documentation on how it works. capDL generalises levels
+ * to nat and page table types to all types that are used by any of the seL4 architectures.
  *)
 
 datatype cdl_cap =
@@ -116,9 +128,9 @@ datatype cdl_cap =
 
   (* Kernel object capabilities *)
   | UntypedCap bool cdl_object_set cdl_object_set
-  | EndpointCap cdl_object_id cdl_badge "cdl_right set"
-  | NotificationCap cdl_object_id cdl_badge "cdl_right set"
-  | ReplyCap cdl_object_id "cdl_right set" (* The id of the tcb of the target thread *)
+  | EndpointCap cdl_object_id (cap_badge : cdl_badge) (cdl_cap_rights : "cdl_right set")
+  | NotificationCap cdl_object_id (cap_badge : cdl_badge) (cdl_cap_rights : "cdl_right set")
+  | ReplyCap cdl_object_id (cdl_cap_rights : "cdl_right set") (* The id of the tcb of the target thread *)
   | MasterReplyCap cdl_object_id
   | CNodeCap cdl_object_id cdl_cap_guard cdl_cap_guard_size cdl_size_bits
   | TcbCap cdl_object_id
@@ -145,9 +157,15 @@ datatype cdl_cap =
   | SGISignalCap sgi_irq sgi_target
 
   (* Virtual memory capabilties *)
-  | FrameCap bool cdl_object_id "cdl_right set" nat cdl_frame_cap_type "cdl_mapped_addr option"
-  | PageTableCap cdl_object_id cdl_frame_cap_type "cdl_mapped_addr option"
-  | PageDirectoryCap cdl_object_id cdl_frame_cap_type "cdl_asid option"
+  | FrameCap bool (cdl_obj : cdl_object_id)
+                  (cdl_cap_rights : "cdl_right set")
+                  (cdl_frame_sz : nat)
+                  (cdl_frame_cap_type : cdl_frame_cap_type)
+                  (cdl_mapped_addr : "cdl_mapped_addr option")
+  | PageTableCap (cdl_cap_pt_type : cdl_pt_type)
+                 (cdl_obj : cdl_object_id)
+                 (cdl_frame_cap_type : cdl_frame_cap_type)
+                 (cdl_mapped_addr : "cdl_mapped_addr option")
   | AsidControlCap
   | AsidPoolCap cdl_object_id "cdl_cnode_index"
 
@@ -220,12 +238,6 @@ record cdl_cnode =
 record cdl_asid_pool =
   cdl_asid_pool_caps :: cdl_cap_map
 
-record cdl_page_table =
-  cdl_page_table_caps :: cdl_cap_map
-
-record cdl_page_directory =
-  cdl_page_directory_caps :: cdl_cap_map
-
 (* Extra "frame fill" data. The executable initialiser requires this
  * so that it can load pages for components. For now, we only support
  * FileData, which is copied from a linked cpio archive. *)
@@ -254,8 +266,7 @@ datatype cdl_object =
   | Tcb cdl_tcb
   | CNode cdl_cnode
   | AsidPool cdl_asid_pool
-  | PageTable cdl_page_table
-  | PageDirectory cdl_page_directory
+  | PageTable (cdl_pt_type : cdl_pt_type) (cdl_pt_map : cdl_cap_map)
   | Frame cdl_frame
   | Untyped
   | IRQNode cdl_irq_node
@@ -320,22 +331,23 @@ where
       | CNode _ \<Rightarrow> CNodeType
       | IRQNode _ \<Rightarrow> IRQNodeType
       | AsidPool _ \<Rightarrow> AsidPoolType
-      | PageTable _ \<Rightarrow> PageTableType
-      | PageDirectory _ \<Rightarrow> PageDirectoryType
+      | PageTable l _ \<Rightarrow> PageTableType l
       | Frame f \<Rightarrow> FrameType (cdl_frame_size_bits f)
       | VCPU \<Rightarrow> VCPUType"
 
 lemmas object_type_simps = object_type_def[split_simps cdl_object.split]
 
 definition
-  asid_high_bits :: nat where (* FIXME AARCH64 *)
-  "asid_high_bits \<equiv> 7"
+  asid_high_bits :: nat where
+  "asid_high_bits \<equiv> LENGTH(asid_high_len)"
+
 definition
   asid_low_bits :: nat where
-  "asid_low_bits \<equiv> 10 :: nat"
+  "asid_low_bits \<equiv> LENGTH(asid_low_len)"
+
 definition
   asid_bits :: nat where
-  "asid_bits \<equiv> 17 :: nat"
+  "asid_bits \<equiv> asid_high_bits + asid_low_bits"
 
 (*
  * Each TCB contains a number of cap slots, each with a specific
@@ -385,8 +397,7 @@ where
   | "cap_objects (IOSpaceCap x) = {x}"
   | "cap_objects (IOPortsCap x _) = {x}"
   | "cap_objects (AsidPoolCap x _) = {x}"
-  | "cap_objects (PageDirectoryCap x _ _) = {x}"
-  | "cap_objects (PageTableCap x _ _) = {x}"
+  | "cap_objects (PageTableCap _ x _ _) = {x}"
   | "cap_objects (FrameCap _ x _ _ _ _) = {x}"
   | "cap_objects (TcbCap x) = {x}"
   | "cap_objects (CNodeCap x _ _ _) = {x}"
@@ -431,8 +442,7 @@ lemma cap_object_simps[simp]:
   "cap_object (IOSpaceCap x) = x"
   "cap_object (IOPortsCap x a) = x"
   "cap_object (AsidPoolCap x b) = x"
-  "cap_object (PageDirectoryCap x c d) = x"
-  "cap_object (PageTableCap x e f) = x"
+  "cap_object (PageTableCap pt_t x e f) = x"
   "cap_object (FrameCap dev x g h i j) = x"
   "cap_object (TcbCap x) = x"
   "cap_object (CNodeCap x k l sz) = x"
@@ -447,33 +457,24 @@ lemma cap_object_simps[simp]:
   "cap_object (BoundNotificationCap x) = x"
   "cap_object (VCPUCap x) = x"
   by (simp_all add:cap_object_def Nitpick.The_psimp cap_has_object_def)
-      (metis (full_types) LeastI)+
+     (metis (full_types) LeastI)+
 
-primrec (nonexhaustive) cap_badge :: "cdl_cap \<Rightarrow> cdl_badge"
-where
-    "cap_badge (NotificationCap _ x _) = x"
-  | "cap_badge (EndpointCap _ x _) = x"
-
-definition
-  update_cap_badge :: "cdl_badge \<Rightarrow> cdl_cap \<Rightarrow> cdl_cap"
-where
+definition update_cap_badge :: "cdl_badge \<Rightarrow> cdl_cap \<Rightarrow> cdl_cap" where
   "update_cap_badge x c \<equiv> case c of
-      NotificationCap f1 _ f3 \<Rightarrow> NotificationCap f1 x f3
-    | EndpointCap f1 _ f3      \<Rightarrow> EndpointCap f1 x f3
-    | _ \<Rightarrow> c"
+     NotificationCap f1 _ f3 \<Rightarrow> NotificationCap f1 x f3
+   | EndpointCap f1 _ f3     \<Rightarrow> EndpointCap f1 x f3
+   | _ \<Rightarrow> c"
 
 definition all_cdl_rights :: "cdl_right set" where
   "all_cdl_rights = {Read, Write, Grant, GrantReply}"
 
-definition
-  cap_rights :: "cdl_cap \<Rightarrow> cdl_right set"
-where
+definition cap_rights :: "cdl_cap \<Rightarrow> cdl_right set" where
   "cap_rights c \<equiv> case c of
-      FrameCap _ _ x _ _ _ \<Rightarrow> x
-    | NotificationCap _ _ x \<Rightarrow> x
-    | EndpointCap _ _ x \<Rightarrow> x
-    | ReplyCap _ x \<Rightarrow> x
-    | _ \<Rightarrow> all_cdl_rights"
+     FrameCap _ _ _  _ _ _ \<Rightarrow> cdl_cap_rights c
+   | NotificationCap _ _ _ \<Rightarrow> cdl_cap_rights c
+   | EndpointCap _ _ _     \<Rightarrow> cdl_cap_rights c
+   | ReplyCap _ _          \<Rightarrow> cdl_cap_rights c
+   | _ \<Rightarrow> all_cdl_rights"
 
 definition
   update_cap_rights :: "cdl_right set \<Rightarrow> cdl_cap \<Rightarrow> cdl_cap"
@@ -490,7 +491,7 @@ definition
 where
  "update_mapping_cap_status r c \<equiv> case c of
       FrameCap dev f1 f2 f3 _ f4 \<Rightarrow> FrameCap dev f1 f2 f3 r f4
-    | PageTableCap pt1 _ pt2 \<Rightarrow> PageTableCap pt1 r pt2
+    | PageTableCap l pt1 _ pt2 \<Rightarrow> PageTableCap l pt1 r pt2
     | _ \<Rightarrow> c"
 
 primrec (nonexhaustive) cap_guard :: "cdl_cap \<Rightarrow> cdl_cap_guard"
@@ -527,7 +528,7 @@ definition
 where
   "cap_vmattrs cap \<equiv> case cap of
       FrameCap _ _ _ _ (Fake attr) _ \<Rightarrow> attr
-    | PageTableCap _ (Fake attr) _ \<Rightarrow> attr"
+    | PageTableCap _ _ (Fake attr) _ \<Rightarrow> attr"
 
 definition
   frame_cap_size :: "cdl_cap \<Rightarrow> cdl_size_bits"
@@ -541,8 +542,7 @@ definition
   object_slots :: "cdl_object \<Rightarrow> cdl_cap_map"
 where
   "object_slots obj \<equiv> case obj of
-    PageDirectory x \<Rightarrow> cdl_page_directory_caps x
-  | PageTable x \<Rightarrow> cdl_page_table_caps x
+    PageTable _ x \<Rightarrow> x
   | AsidPool x \<Rightarrow> cdl_asid_pool_caps x
   | CNode x \<Rightarrow> cdl_cnode_caps x
   | Tcb x \<Rightarrow> cdl_tcb_caps x
@@ -553,8 +553,7 @@ definition
   update_slots :: "cdl_cap_map \<Rightarrow> cdl_object \<Rightarrow> cdl_object"
 where
   "update_slots new_val obj \<equiv> case obj of
-    PageDirectory x \<Rightarrow> PageDirectory (x\<lparr>cdl_page_directory_caps := new_val\<rparr>)
-  | PageTable x \<Rightarrow> PageTable (x\<lparr>cdl_page_table_caps := new_val\<rparr>)
+    PageTable l x \<Rightarrow> PageTable l new_val
   | AsidPool x \<Rightarrow> AsidPool (x\<lparr>cdl_asid_pool_caps := new_val\<rparr>)
   | CNode x \<Rightarrow> CNode (x\<lparr>cdl_cnode_caps := new_val\<rparr>)
   | Tcb x \<Rightarrow> Tcb (x\<lparr>cdl_tcb_caps := new_val\<rparr>)
@@ -565,8 +564,7 @@ definition
   has_slots :: "cdl_object \<Rightarrow> bool"
 where
   "has_slots obj \<equiv> case obj of
-    PageDirectory _ \<Rightarrow> True
-  | PageTable _ \<Rightarrow> True
+    PageTable _ _ \<Rightarrow> True
   | AsidPool _ \<Rightarrow> True
   | CNode _ \<Rightarrow> True
   | Tcb _ \<Rightarrow> True
@@ -606,8 +604,7 @@ definition cap_type :: "cdl_cap \<Rightarrow> cdl_object_type option" where
   | TcbCap _               \<Rightarrow> Some TcbType
   | CNodeCap _ _ _ _       \<Rightarrow> Some CNodeType
   | AsidPoolCap _ _        \<Rightarrow> Some AsidPoolType
-  | PageTableCap _ _ _     \<Rightarrow> Some PageTableType
-  | PageDirectoryCap _ _ _ \<Rightarrow> Some PageDirectoryType
+  | PageTableCap t _ _ _   \<Rightarrow> Some (PageTableType t)
   | FrameCap _ _ _ f _ _   \<Rightarrow> Some (FrameType f)
   | IrqHandlerCap _        \<Rightarrow> Some IRQNodeType
   | VCPUCap _              \<Rightarrow> Some VCPUType
@@ -620,8 +617,10 @@ abbreviation "is_ntfn_cap cap       \<equiv> cap_type cap = Some NotificationTyp
 abbreviation "is_tcb_cap cap        \<equiv> cap_type cap = Some TcbType"
 abbreviation "is_cnode_cap cap      \<equiv> cap_type cap = Some CNodeType"
 abbreviation "is_asidpool_cap cap   \<equiv> cap_type cap = Some AsidPoolType"
-abbreviation "is_pt_cap cap         \<equiv> cap_type cap = Some PageTableType"
-abbreviation "is_pd_cap cap         \<equiv> cap_type cap = Some PageDirectoryType"
+abbreviation "is_table_cap cap      \<equiv> \<exists>l. cap_type cap = Some (PageTableType l)"
+abbreviation "is_pt_type_cap l cap  \<equiv> cap_type cap = Some (PageTableType l)"
+abbreviation "is_pt_cap             \<equiv> is_pt_type_cap PT"
+abbreviation "is_pd_cap             \<equiv> is_pt_type_cap PD"
 abbreviation "is_frame_cap cap      \<equiv> \<exists>sz. cap_type cap = Some (FrameType sz)"
 abbreviation "is_irqhandler_cap cap \<equiv> cap_type cap = Some IRQNodeType"
 definition   "is_irqcontrol_cap cap \<equiv> cap = IrqControlCap"
@@ -634,12 +633,14 @@ lemma cap_type_simps[simp]:
   "is_tcb_cap        (TcbCap h)"
   "is_cnode_cap      (CNodeCap j k l m)"
   "is_asidpool_cap   (AsidPoolCap n p)"
-  "is_pd_cap         (PageDirectoryCap r s t)"
-  "is_pt_cap         (PageTableCap u v w)"
+  "is_pt_cap         (PageTableCap PT u v w)"
+  "is_pd_cap         (PageTableCap PD u v w)"
+  "is_table_cap      (PageTableCap t u v w)"
+  "is_pt_type_cap t  (PageTableCap t u v w)"
   "is_frame_cap      (FrameCap dev a1 a2 a3 a4 a5)"
   "is_irqhandler_cap (IrqHandlerCap a6)"
   "is_vcpu_cap       (VCPUCap b)"
-  "cap_type (FrameCap dev obj_id rights sz rs asid) = Some (FrameType sz)"
+  "cap_type          (FrameCap dev obj_id rights sz rs asid) = Some (FrameType sz)"
   by (clarsimp simp: cap_type_def)+
 
 abbreviation cap_has_type :: "cdl_cap \<Rightarrow> bool" where
@@ -729,6 +730,56 @@ where
 definition default_frame_fill_data :: "cdl_frame_fill list" where
   "default_frame_fill_data \<equiv> []"
 
+(* vsroot_size_index is so far only used on AARCH64, so we are directly making use of AARCH64
+   specific config values. If we start using vsroot_size_index for other architectures, this
+   will need a case distinction on architecture. *)
+definition vsroot_size_index :: nat where
+  "vsroot_size_index \<equiv> if config_ARM_PA_SIZE_BITS_40 then 10 else pt_size_index"
+
+definition pt_type_index_bits :: "cdl_pt_type \<Rightarrow> nat" where
+  "pt_type_index_bits pt_t \<equiv>
+     case pt_t of
+       PT     \<Rightarrow> pt_size_index
+     | PD     \<Rightarrow> pd_size_index
+     | VSROOT \<Rightarrow> vsroot_size_index
+     | PDPT   \<Rightarrow> pt_size_index
+     | PML4   \<Rightarrow> pt_size_index"
+
+definition
+  "max_pt_level \<equiv>
+     case cdl_ARCH of
+       AARCH32 \<Rightarrow> 1
+     | AARCH64 \<Rightarrow> if config_ARM_PA_SIZE_BITS_40 then 3 else 4
+     | RISCV32 \<Rightarrow> 1
+     | RISCV64 \<Rightarrow> 3
+     | IA32    \<Rightarrow> 1
+     | X64     \<Rightarrow> 3"
+
+definition cdl_level_type :: "nat \<Rightarrow> cdl_pt_type" where
+  "cdl_level_type \<equiv>
+     case cdl_ARCH of
+       AARCH32 \<Rightarrow> (\<lambda>_. PT) (max_pt_level := PD)
+     | AARCH64 \<Rightarrow> (\<lambda>_. PT) (max_pt_level := vspace_type)
+     | RISCV32 \<Rightarrow> (\<lambda>_. PT)
+     | RISCV64 \<Rightarrow> (\<lambda>_. PT)
+     | IA32    \<Rightarrow> (\<lambda>_. PT) (max_pt_level := PD)
+     | X64     \<Rightarrow> (\<lambda>_. PT) (1 := PD, 2 := PDPT, max_pt_level := PML4)"
+
+lemma max_pt_level_0[simp]:
+  "cdl_level_type 0 = PT"
+  unfolding cdl_level_type_def max_pt_level_def
+  by (clarsimp split: cdl_arch.split)
+
+lemma max_pt_level_vspace_type[simp]:
+  "cdl_level_type max_pt_level = vspace_type"
+  unfolding cdl_level_type_def max_pt_level_def vspace_type_def
+  by (clarsimp split: cdl_arch.split)
+
+abbreviation pt_translation_bits :: "nat \<Rightarrow> nat" where
+  "pt_translation_bits level \<equiv> pt_type_index_bits (cdl_level_type level)"
+
+lemmas pt_translation_bits_def = pt_type_index_bits_def cdl_level_type_def
+
 (* Return a newly constructed object of the given type. *)
 definition
   default_object :: "cdl_object_type \<Rightarrow> nat \<Rightarrow> domain \<Rightarrow> cdl_object option"
@@ -741,8 +792,7 @@ where
       | TcbType \<Rightarrow> Some (Tcb (default_tcb current_domain))
       | CNodeType \<Rightarrow> Some (CNode (empty_cnode sz))
       | AsidPoolType \<Rightarrow> Some (AsidPool \<lparr> cdl_asid_pool_caps = empty_cap_map asid_low_bits \<rparr>)
-      | PageTableType \<Rightarrow> Some (PageTable \<lparr> cdl_page_table_caps = empty_cap_map pt_size_index \<rparr>)
-      | PageDirectoryType \<Rightarrow> Some (PageDirectory \<lparr> cdl_page_directory_caps = empty_cap_map pd_size_index \<rparr>)
+      | PageTableType t \<Rightarrow> Some (PageTable t (empty_cap_map (pt_type_index_bits t)))
       | FrameType sz \<Rightarrow> Some (Frame \<lparr> cdl_frame_size_bits = sz,
                                       cdl_frame_fills = default_frame_fill_data \<rparr>)
       | IRQNodeType \<Rightarrow> Some (IRQNode empty_irq_node)
@@ -764,8 +814,7 @@ where
       | IRQNodeType \<Rightarrow> IrqHandlerCap undefined
       | UntypedType \<Rightarrow> UntypedCap dev id_set id_set
       | AsidPoolType \<Rightarrow> AsidPoolCap (pick id_set) 0
-      | PageTableType \<Rightarrow> PageTableCap (pick id_set) Real None
-      | PageDirectoryType \<Rightarrow> PageDirectoryCap (pick id_set) Real None
+      | PageTableType l \<Rightarrow> PageTableCap l (pick id_set) Real None
       | FrameType frame_size \<Rightarrow> FrameCap dev (pick id_set) {Read, Write} frame_size Real None
       | VCPUType \<Rightarrow> VCPUCap (pick id_set)"
 
